src/FcEtt/ett_value.v
@@ -1,6 +1,6 @@
 Set Bullet Behavior "Strict Subproofs".
 Set Implicit Arguments.
-
+Require Export FcEtt.ett_inf_cs.
 Require Export FcEtt.tactics.
 Require Export FcEtt.imports.
 Require Export FcEtt.ett_inf.
@@ -14,7 +14,6 @@ Require Import FcEtt.ext_wf.
 Import ext_wf.
 
 Require Import FcEtt.utils.
-Require Import FcEtt.erase_syntax.
 Require Export FcEtt.toplevel.
 
 
@@ -25,8 +24,8 @@ Require Export FcEtt.toplevel.
 (* Values and CoercedValues *)
 
 Lemma tm_subst_tm_tm_Value_mutual :
-  (forall v,  CoercedValue v -> forall b x,  lc_tm b -> CoercedValue (tm_subst_tm_tm b x v)) /\
-  (forall v, Value v -> forall b x,  lc_tm b -> Value (tm_subst_tm_tm b x v)).
+  (forall R v,  CoercedValue R v -> forall b x,  lc_tm b -> CoercedValue R (tm_subst_tm_tm b x v)) /\
+  (forall R v, Value R v -> forall b x,  lc_tm b -> Value R (tm_subst_tm_tm b x v)).
 Proof.
   apply CoercedValue_Value_mutual; simpl.
   all: try solve [inversion 1 | econstructor; eauto]; eauto.
@@ -39,11 +38,11 @@ Proof.
     match goal with [H: lc_tm (?a1 ?a2), K : lc_tm ?b |- _ ] =>
                     move: (tm_subst_tm_tm_lc_tm _ _ x H K) => h0; auto end].
 
-  - intros L R a v H b x H0.
+  - intros L R R1 a v H b x H0.
     econstructor; eauto.
     instantiate (1 := L \u singleton x) => x0 h0.
     rewrite tm_subst_tm_tm_open_tm_wrt_tm_var; auto.
-  - intros L A R a l c H b x H0.
+  - intros L R A R1 a l c H b x H0.
     econstructor; eauto.
     apply tm_subst_tm_tm_lc_tm; auto.
     instantiate (1 := L \u singleton x) => x0 h0.
@@ -51,38 +50,38 @@ Proof.
 Qed.
 
 Lemma Value_tm_subst_tm_tm :
-  (forall v b x, Value v -> lc_tm b -> Value (tm_subst_tm_tm b x v)).
+  (forall R v b x, Value R v -> lc_tm b -> Value R (tm_subst_tm_tm b x v)).
 Proof.
-  intros v b x H H0.
+  intros R v b x H H0.
   apply tm_subst_tm_tm_Value_mutual; auto.
 Qed.
 
 Lemma CoercedValue_tm_subst_tm_tm :
-  (forall v b x, CoercedValue v -> lc_tm b -> CoercedValue (tm_subst_tm_tm b x v)).
+  (forall R v b x, CoercedValue R v -> lc_tm b -> CoercedValue R (tm_subst_tm_tm b x v)).
 Proof.
-  intros v b x H H0.
+  intros R v b x H H0.
   destruct (tm_subst_tm_tm_Value_mutual); auto.
 Qed.
 
 (* ------------------------------------------------- *)
 
-Lemma Value_UAbsIrrel_exists : ∀ x (a : tm) R,
+Lemma Value_UAbsIrrel_exists : ∀ x (a : tm) R R1,
     x `notin` fv_tm a
-    → (Value (open_tm_wrt_tm a (a_Var_f x)))
-    → Value (a_UAbs Irrel R a).
+    → (CoercedValue R (open_tm_wrt_tm a (a_Var_f x)))
+    → Value R (a_UAbs Irrel R1 a).
 Proof.
   intros.
   eapply (Value_UAbsIrrel ({{x}})); eauto.
   intros.
   rewrite (tm_subst_tm_tm_intro x); eauto.
-  eapply Value_tm_subst_tm_tm; auto.
+  eapply CoercedValue_tm_subst_tm_tm; auto.
 Qed.
 
-Lemma Value_AbsIrrel_exists : ∀ x (A a : tm) R,
+Lemma Value_AbsIrrel_exists : ∀ x (A a : tm) R R1,
     x `notin` fv_tm a
     -> lc_tm A
-    → (CoercedValue (open_tm_wrt_tm a (a_Var_f x)))
-    → Value (a_Abs Irrel A R a).
+    → (CoercedValue R (open_tm_wrt_tm a (a_Var_f x)))
+    → Value R (a_Abs Irrel A R1 a).
 Proof.
   intros.
   eapply (Value_AbsIrrel ({{x}})); eauto.
@@ -94,8 +93,8 @@ Qed.
 (* ----- *)
 
 Lemma co_subst_co_tm_Value_mutual :
-  (forall v,  CoercedValue v -> forall b x,  lc_co b -> CoercedValue (co_subst_co_tm b x v)) /\
-  (forall v, Value v -> forall b x,  lc_co b -> Value (co_subst_co_tm b x v)).
+  (forall R v,  CoercedValue R v -> forall b x,  lc_co b -> CoercedValue R (co_subst_co_tm b x v)) /\
+  (forall R v, Value R v -> forall b x,  lc_co b -> Value R (co_subst_co_tm b x v)).
 Proof.
   apply CoercedValue_Value_mutual; simpl.
   all: try solve [inversion 1 | econstructor; eauto]; eauto.
@@ -125,16 +124,16 @@ Proof.
 Qed.
 
 Lemma Value_co_subst_co_tm :
-  (forall v b x, Value v -> lc_co b -> Value (co_subst_co_tm b x v)).
+  (forall R v b x, Value R v -> lc_co b -> Value R (co_subst_co_tm b x v)).
 Proof.
-  intros v b x H H0.
+  intros R v b x H H0.
   apply co_subst_co_tm_Value_mutual; auto.
 Qed.
 
 Lemma CoercedValue_co_subst_co_tm :
-  (forall v b x, CoercedValue v -> lc_co b -> CoercedValue (co_subst_co_tm b x v)).
+  (forall R v b x, CoercedValue R v -> lc_co b -> CoercedValue R (co_subst_co_tm b x v)).
 Proof.
-  intros v b x H H0.
+  intros R v b x H H0.
   destruct (co_subst_co_tm_Value_mutual); auto.
 Qed.
 
